code/Yazi.Huffman.fsti
@@ -67,3 +67,4 @@ val static_bl_desc: B.pointer static_tree_desc
 
 [@CMacro]
 let end_block = 256ul
+
