code/Yazi.Tree.fst
@@ -1,0 +1,180 @@
+module Yazi.Tree
+
+module B = LowStar.Buffer
+module CB = LowStar.ConstBuffer
+module HS = FStar.HyperStack
+module Seq = FStar.Seq
+module SH = Spec.Tree.Heap
+module ST = FStar.HyperStack.ST
+module U16 = FStar.UInt16
+module U32 = FStar.UInt32
+module U8 = FStar.UInt8
+
+open FStar.Mul
+open Lib.Seq
+open LowStar.BufferOps
+open Yazi.Deflate.Constants
+open Yazi.Tree.Types
+
+inline_for_extraction
+let get_heap_len (ts: tree_state_t): ST.Stack U32.t
+  (requires fun h -> SH.tree_state_live h ts)
+  (ensures fun h0 res h1 ->
+    B.modifies B.loc_none h0 h1 /\
+    U32.v res == SH.get_heap_len h1 ts) =
+  (CB.index ts.ctx 0ul).state.(0ul)
+
+inline_for_extraction
+let set_heap_len (ts: tree_state_t) (a: U32.t): ST.Stack unit
+  (requires fun h -> SH.tree_state_live h ts)
+  (ensures fun h0 _ h1 ->
+    B.modifies (B.loc_buffer ((CB.as_seq h0 ts.ctx).[0]).state) h0 h1 /\
+    SH.get_heap_len h1 ts == U32.v a /\
+    SH.get_heap_max h0 ts == SH.get_heap_max h1 ts) =
+  (CB.index ts.ctx 0ul).state.(0ul) <- a
+
+inline_for_extraction
+let get_heap_max (ts: tree_state_t): ST.Stack U32.t
+  (requires fun h -> SH.tree_state_live h ts)
+  (ensures fun h0 res h1 ->
+    B.modifies B.loc_none h0 h1 /\
+    U32.v res == SH.get_heap_max h0 ts) =
+  (CB.index ts.ctx 0ul).state.(1ul)
+
+inline_for_extraction
+let set_heap_max (ts: tree_state_t) (a: U32.t): ST.Stack unit
+  (requires fun h -> SH.tree_state_live h ts)
+  (ensures fun h0 _ h1 ->
+    B.modifies (B.loc_buffer ((CB.as_seq h0 ts.ctx).[0]).state) h0 h1 /\
+    SH.get_heap_max h1 ts == U32.v a /\
+    SH.get_heap_len h0 ts == SH.get_heap_len h1 ts) =
+  (CB.index ts.ctx 0ul).state.(1ul) <- a
+
+inline_for_extraction
+let smaller (ts: tree_state_t) (n m: U32.t): ST.Stack bool
+  (requires fun h ->
+    SH.tree_state_live h ts /\
+    (let ts = SH.g_tree_state h ts in
+    SH.heap_elems_wf ts /\ SH.is_tree_index ts n /\ SH.is_tree_index ts m))
+  (ensures fun h0 res h1 ->
+    let ts = SH.g_tree_state h0 ts in
+    B.modifies B.loc_none h0 h1 /\
+    res == SH.smaller ts n m) =
+  let tree = (CB.index ts.ctx 0ul).tree in
+  let nfc = (tree.(n)).freq_or_code in
+  let mfc = (tree.(m)).freq_or_code in
+  if nfc `U16.lt` mfc then
+    true
+  else if nfc `U16.eq` mfc then
+    let depth = (CB.index ts.ctx 0ul).depth in
+    let dn = depth.(n) in
+    let dm = depth.(m) in
+    if dn `U8.lt` dm then
+      true
+    else if dn `U8.eq` dm then
+      n `U32.lte` m
+    else
+      false
+  else
+    false
+
+inline_for_extraction
+let smallest (ts: tree_state_t) (root: Ghost.erased U32.t) (i hole: U32.t): ST.Stack U32.t
+  (requires fun h ->
+    SH.tree_state_live h ts /\
+    SH.heap_elems_wf (SH.g_tree_state h ts) /\
+    SH.insertion_pre_cond (SH.g_tree_state h ts) root i hole /\
+    U32.v hole <= SH.get_heap_len h ts / 2)
+  (ensures fun h0 res h1 ->
+    B.modifies B.loc_none h0 h1 /\
+    res == SH.smallest (SH.g_tree_state h0 ts) root i hole) =
+  let open U32 in
+  let l = hole *^ 2ul in let r = l +^ 1ul in
+  let le = (CB.index ts.ctx 0ul).heap.(l) in
+
+  let heap_len = get_heap_len ts in
+  [@inline_let] let smaller = smaller ts in
+  if r >^ heap_len then
+    if i `smaller` le then 0ul else l
+  else
+    let re = (CB.index ts.ctx 0ul).heap.(r) in
+    if i `smaller` le then
+      if i `smaller` re then 0ul else r
+    else
+      if le `smaller` re then l else r
+
+#push-options "--z3refresh --z3rlimit 128 --fuel 1 --ifuel 0 --z3seed 111"
+inline_for_extraction
+let rec do_pqdownheap
+  (h0: Ghost.erased HS.mem) (ts: tree_state_t)
+  (root: Ghost.erased U32.t) (i hole: U32.t):
+  ST.Stack unit
+  (requires fun h1 ->
+    SH.tree_state_live h0 ts /\ SH.tree_state_live h1 ts /\
+    B.modifies (B.loc_buffer ((CB.as_seq h1 ts.ctx).[0]).heap) h0 h1 /\
+    SH.do_pqdownheap_pre (SH.g_tree_state h0 ts) (SH.g_tree_state h1 ts) root i hole)
+  (ensures fun h1 _ h2 ->
+    let open SH in
+    let ts0 = SH.g_tree_state h0 ts in
+    let ts1 = SH.g_tree_state h1 ts in
+    SH.tree_state_live h2 ts /\
+    B.modifies (B.loc_buffer ((CB.as_seq h1 ts.ctx).[0]).heap) h1 h2 /\
+    SH.g_tree_state h2 ts == SH.do_pqdownheap ts0 ts1 root i hole)
+  (decreases SH.get_heap_len h0 ts / 2 - U32.v hole) =
+  let open U32 in
+  let heap_len = get_heap_len ts in
+  let heap = (CB.index ts.ctx 0ul).heap in
+  if hole >^ heap_len /^ 2ul then
+    heap.(hole) <- i
+  else
+    let s = smallest ts root i hole in
+    if s = 0ul then
+      heap.(hole) <- i
+    else begin
+      heap.(hole) <- heap.(s);
+      do_pqdownheap h0 ts root i s
+    end
+
+inline_for_extraction
+let pqdownheap (ts: tree_state_t) (i: U32.t): ST.Stack unit
+  (requires fun h ->
+    SH.tree_state_live h ts /\
+    SH.is_internal_index (SH.g_tree_state h ts) i /\
+    SH.pqdownheap_pre (SH.g_tree_state h ts) i)
+  (ensures fun h0 _ h1 ->
+    B.modifies (B.loc_buffer ((CB.as_seq h0 ts.ctx).[0]).heap) h0 h1 /\
+    SH.g_tree_state h1 ts == SH.pqdownheap (SH.g_tree_state h0 ts) i) =
+  do_pqdownheap (ST.get ()) ts i (CB.index ts.ctx 0ul).heap.(i) i
+#pop-options
+
+#push-options "--z3refresh --z3rlimit 128 --fuel 0 --ifuel 0 --query_stats"
+inline_for_extraction
+let pqremove (ts: tree_state_t):
+  ST.Stack U32.t
+  (requires fun h ->
+    SH.tree_state_live h ts /\
+    SH.heap_wf (SH.g_tree_state h ts) /\
+    SH.get_heap_len h ts > 1)
+  (ensures fun h0 top h1 ->
+    B.modifies (
+      B.loc_buffer ((CB.as_seq h0 ts.ctx).[0]).heap `B.loc_union`
+      B.loc_buffer ((CB.as_seq h0 ts.ctx).[0]).state
+    ) h0 h1 /\
+    SH.tree_state_live h1 ts /\
+    SH.g_tree_state h1 ts == SH.pqremove (SH.g_tree_state h0 ts) /\
+    (SH.g_tree_state h0 ts <: SH.tree_state).heap.[1] == top) =
+  let h0 = ST.get () in
+  SH.lemma_heap_wf_pqremove (SH.g_tree_state h0 ts);
+  let open U32 in
+  let heap_len = get_heap_len ts in
+  let heap_max = get_heap_max ts in
+  let heap = (CB.index ts.ctx 0ul).heap in
+  let top = heap.(1ul) in
+  let bot = heap.(heap_len) in
+  heap.(heap_max -^ 1ul) <- top;
+  heap.(1ul) <- bot;
+  set_heap_len ts (heap_len -^ 1ul);
+  set_heap_max ts (heap_max -^ 1ul);  
+  if heap_len -^ 1ul >=^ 2ul then pqdownheap ts 1ul;
+  top
+#pop-options
