specs/Spec.Heap.Lemmas.fst
@@ -1,0 +1,198 @@
+module Spec.Heap.Lemmas
+
+(** Lemmas to verify that smaller() is a total order relation. **)
+let lemma_smaller_asym (ts: heap_elems_wf_ts) (i j: U32.t): Lemma
+  (requires
+    is_tree_index ts i /\ is_tree_index ts j /\
+    smaller ts i j /\ smaller ts j i)
+  (ensures i == j) = ()
+
+let lemma_smaller_trans (ts: heap_elems_wf_ts) (a b c: U32.t): Lemma
+  (requires
+    is_tree_index ts a /\ is_tree_index ts b /\ is_tree_index ts c /\
+    smaller ts a b /\ smaller ts b c)
+  (ensures smaller ts a c) = ()
+
+let lemma_smaller_comp (ts: heap_elems_wf_ts) (i j: U32.t): Lemma
+  (requires is_tree_index ts i /\ is_tree_index ts j)
+  (ensures smaller ts i j \/ smaller ts j i) = ()
+
+let lemma_heap_seq_upd_perm ts0 ts1 =
+  assert(equal
+    (Seq.slice ts0.heap (ts0.heap_len + 1) (U32.v heap_size))
+    (Seq.slice ts1.heap (ts0.heap_len + 1) (U32.v heap_size)));
+  permutation_split ts0.heap ts1.heap 1 (ts0.heap_len + 1)
+
+let rec lemma_heap_sorted' (ts0 ts1: heap_elems_wf_ts) (i: nat{
+  ts0.heap_max <= i /\ i <= U32.v heap_size
+}): Lemma
+  (requires
+    ts1 == {ts0 with heap = ts1.heap} /\
+    heap_sorted' ts0 i /\
+    non_heap_unmodified ts0.heap ts1.heap ts0.heap_len)
+  (ensures heap_sorted' ts1 i)
+  (decreases U32.v heap_size - i) =
+  match U32.v heap_size - i with
+  | 0 -> ()
+  | _ -> lemma_heap_sorted' ts0 ts1 (i + 1)
+
+let lemma_non_heap_unmodified ts0 ts1 =
+  assert(equal (sorted_seq ts0) (sorted_seq ts1));
+  match U32.v heap_size - ts0.heap_max with
+  | 0 -> ()
+  | _ -> lemma_heap_sorted' ts0 ts1 ts0.heap_max
+
+let rec log2 (a: pos): Tot (n: nat{
+  pow2 n <= a /\ a < pow2 (n + 1)
+}) = if a = 1 then 0 else 1 + log2 (a / 2)
+
+let rec log2_pow2_lt (a: pos) (n: nat): Lemma
+  (requires n < log2 a)
+  (ensures pow2 n < a) =
+  match n with
+  | 0 -> ()
+  | _ -> log2_pow2_lt (a / 2) (n - 1)
+
+let rec log2_pow2_gt (a: pos) (n: pos): Lemma
+  (requires a < pow2 n)
+  (ensures log2 a < n) =
+  match (a, n) with
+  | (1, _) | (_, 1) -> ()
+  | _ -> log2_pow2_gt (a / 2) (n - 1)
+
+let rec ancestor (a: pos) (i: pos{i <= log2 a}): Tot (res: pos{res < a}) =
+  if i > 1 then ancestor (a / 2) (i - 1) else a / 2
+
+let rec lemma_ancestor_next (a: pos) (i: pos{1 < i /\ i <= log2 a}): Lemma
+  (ensures ancestor a i == ancestor a (i - 1) / 2) =
+  match i with
+  | 2 -> ()
+  | _ -> lemma_ancestor_next (a / 2) (i - 1)
+
+#push-options "--z3refresh --z3rlimit 128 --fuel 1 --ifuel 0 --z3seed 11"
+/// Generalized version of lemma_heap_wf. Given a heap element whose index is j,
+/// heap.[j] should not smaller than one of its ancestor whose height is smaller than j.
+let rec lemma_partial_wf (height: nat{height < 32}) (ts: heap_elems_wf_ts) (j: pos): Lemma
+  (requires
+    pow2 height < pow2 32 - 1 /\
+    partial_wf ts (U32.uint_to_t (pow2 height)) /\
+    height < log2 j /\ j <= ts.heap_len /\ pow2 height < j)
+  (ensures (
+    let aj = ancestor j (log2 j - height) in
+    pow2 height <= aj /\ aj < pow2 (height + 1) /\
+    smaller ts ts.heap.[aj] ts.heap.[j]))
+  (decreases ts.heap_len - pow2 height) =
+  let aj = ancestor j (log2 j - height) in
+  (* If j's height is height + 1 *)
+  if j < pow2 (height + 2) then begin
+    (* pow2 height < j *)
+    log2_pow2_lt j height;
+    (* log2 j < height + 2 *)
+    log2_pow2_gt j (height + 2);
+    assert(aj * 2 == j \/ aj * 2 + 1 == j)
+    (* Then we have log2 j == height + 1, and the sub-goal can be proven by the
+       hypothesis partial_wf ts (U32.uint_to_t (pow2 height)). *)
+  end else begin
+    (* If j's height is height + n where n > 1. First, we introduce the induction
+       hypothesis. *)
+    lemma_partial_wf (height + 1) ts j;
+    (* Then we have ancestor j (log2 j - height) *)
+    lemma_ancestor_next j (log2 j - height);
+    let aj' = ancestor j (log2 j - (height + 1)) in
+    assert(aj * 2 == aj' \/ aj * 2 + 1 == aj')
+  end
+
+let lemma_heap_wf ts j = if j > 1 then lemma_partial_wf 0 ts j
+#pop-options
+
+#push-options "--z3refresh --z3rlimit 128 --fuel 1 --ifuel 1 --z3seed 111"
+let rec lemma_heap_sorted_sub (ts: heap_elems_wf_ts) (j: nat{
+  ts.heap_max <= j /\ j < U32.v heap_size
+}): Lemma
+  (requires heap_sorted ts)
+  (ensures heap_sorted' ts j) =
+  match j - ts.heap_max with
+  | 0 -> ()
+  | _ -> lemma_heap_sorted_sub ts (j - 1)
+
+private let rec lemma_heap_wf_pqremove_aux
+  (ts0: heap_wf_ts) (ts1: heap_elems_wf_ts)
+  (j: nat{U32.v heap_size > j /\ j > ts1.heap_max}):
+  Lemma
+  (requires
+    ts0.heap_max == ts1.heap_max + 1 /\
+    ts0.tree == ts1.tree /\
+    ts0.depth == ts1.depth /\
+    (forall i. i > ts1.heap_max ==> ts0.heap.[i] == ts1.heap.[i]))
+  (ensures heap_sorted' ts1 j)
+  (decreases U32.v heap_size - j) =
+  if j < U32.v heap_size - 1 then begin
+    lemma_heap_wf_pqremove_aux ts0 ts1 (j + 1);
+    lemma_heap_sorted_sub ts0 j
+  end
+#pop-options
+
+#push-options "--z3refresh --fuel 0 --ifuel 0"
+let lemma_four_seq_perm (#t: eqtype) (top bot mid ss0: seq t) (s: t): Lemma
+  (ensures count s ((bot @| mid) @| (top @| ss0)) == count s ((top @| mid @| bot) @| ss0)) =
+  calc (==) {
+    count s ((bot @| mid) @| (top @| ss0));
+    =={lemma_append_count_aux s (bot @| mid) (top @| ss0)}
+    count s (bot @| mid) + count s (top @| ss0);
+    =={lemma_append_count_aux s bot mid}
+    count s bot + count s mid + count s (top @| ss0);
+    =={lemma_append_count_aux s top ss0}
+    count s bot + count s mid + count s top + count s ss0;
+    =={lemma_append_count_aux s top mid}
+    count s (top @| mid) + count s bot + count s ss0;
+    =={lemma_append_count_aux s (top @| mid) bot}
+    count s ((top @| mid) @| bot) + count s ss0;
+    =={append_assoc top mid bot}
+    count s (top @| mid @| bot) + count s ss0;
+    =={lemma_append_count_aux s (top @| mid @| bot) ss0}
+    count s ((top @| mid @| bot) @| ss0);
+  }
+#pop-options
+
+#push-options "--z3refresh --z3rlimit 256 --fuel 1 --ifuel 0 --z3seed 17"
+let lemma_heap_wf_pqremove ts =
+  let ts' = {
+    ts with
+    heap = upd (upd ts.heap (ts.heap_max - 1) ts.heap.[1]) 1 ts.heap.[ts.heap_len];
+    heap_max = ts.heap_max - 1;
+    heap_len = ts.heap_len - 1;
+  } in
+  let hs0 = heap_seq ts in
+  let hs1 = heap_seq ts' in
+  let top = create 1 hs0.[0] in
+  let mid = slice hs0 1 (length hs0 - 1) in
+  let bot = create 1 (last hs0) in
+  let ss0 = sorted_seq ts in
+  let ss1 = sorted_seq ts' in
+  let es0 = element_seq ts in
+  let es1 = element_seq ts' in
+  calc (==) {
+    es1;
+    =={}
+    hs1 @| ss1;
+    =={assert((bot @| mid) `equal` hs1)}
+    (bot @| mid) @| ss1;
+    =={assert((top @| ss0) `equal` ss1)}
+    (bot @| mid) @| (top @| ss0);
+  };
+  calc (==) {
+    es0;
+    =={}
+    hs0 @| ss0;
+    =={assert((top @| mid @| bot) `equal` hs0)}
+    (top @| mid @| bot) @| ss0;
+  };
+  FStar.Classical.forall_intro (lemma_four_seq_perm top bot mid ss0);
+
+  assert(forall i. {:pattern ts'.heap.[i]} 1 < i /\ i <= ts'.heap_len ==>
+    ts.heap.[i] == ts'.heap.[i]);
+  lemma_heap_wf_forall ts;
+
+  if ts.heap_max < U32.v heap_size then
+    lemma_heap_wf_pqremove_aux ts ts' ts.heap_max
+#pop-options
