specs/Spec.Heap.Lemmas.fsti
@@ -1,0 +1,186 @@
+module Spec.Heap.Lemmas
+
+module U8 = FStar.UInt8
+module U16 = FStar.UInt16
+module U32 = FStar.UInt32
+
+open FStar.Mul
+open FStar.Seq
+open Lib.Seq
+open Yazi.Tree.Types
+open Yazi.Deflate.Constants
+
+/// The tree state type in specification.
+type tree_state = {
+  heap: seq U32.t;
+  tree: seq ct_data;
+  depth: seq U8.t;
+  heap_len: nat;
+  heap_max: nat;
+  tree_len: nat;
+  forest: seq wf_tree;
+}
+
+/// Well-formed tree state. We don't use the tree_state type in the following code.
+type tree_state_wf = res: tree_state{
+  length res.heap == U32.v heap_size /\
+  length res.tree == res.tree_len /\
+  length res.depth == U32.v heap_size /\
+  res.tree_len <= U32.v heap_size
+}
+
+/// The heap indexes: heap_len and heap_max are well-formed.
+let heap_indexes_wf (ts: tree_state) =
+  ts.heap_len < ts.heap_max /\ ts.heap_max <= U32.v heap_size
+
+/// The heap stores the well-formed elements. A heap's elements are well-formed if
+/// all elements in the heap should less than tree_len and heap_size.
+let heap_elems_wf (ts: tree_state_wf) =
+  heap_indexes_wf ts /\
+  (forall i. {:pattern (ts.heap.[i])}
+    0 < i /\ i <= ts.heap_len \/ ts.heap_max <= i /\ i < U32.v heap_size ==>
+    U32.v ts.heap.[i] < ts.tree_len /\ U32.v ts.heap.[i] < 2 * U32.v l_codes + 1)
+
+type heap_elems_wf_ts = ts: tree_state_wf{heap_elems_wf ts}
+
+/// Tree index can be used to index on the tree and depth array.
+let is_tree_index (ts: heap_elems_wf_ts) (i: U32.t) = U32.v i < ts.tree_len
+type tree_index (ts: heap_elems_wf_ts) = i: U32.t{is_tree_index ts i}
+
+/// Tree comparison function. This function is a total order relation.
+let smaller (ts: heap_elems_wf_ts) (i j: tree_index ts): GTot bool =
+  let open U32 in
+  let fi = U16.v (ts.tree.[v i]).freq_or_code in
+  let fj = U16.v (ts.tree.[v j]).freq_or_code in
+  fi < fj ||
+  (fi = fj && U8.v ts.depth.[v i] < U8.v ts.depth.[v j]) ||
+  (fi = fj && U8.v ts.depth.[v i] = U8.v ts.depth.[v j] && v i <= v j)
+
+/// Partial well-formed heap. All elements whose index is large than i should
+/// smaller than their children.
+let partial_wf (ts: tree_state_wf) (i: U32.t{0 < U32.v i}) =
+  heap_elems_wf ts /\
+  (let smaller = smaller ts in
+  let heap = ts.heap in
+  forall (k: nat). U32.v i <= k /\ k <= ts.heap_len / 2 ==> (
+    (heap.[k] `smaller` heap.[k * 2]) /\
+    (k * 2 + 1 <= ts.heap_len ==> heap.[k] `smaller` heap.[k * 2 + 1])))
+
+type partial_wf_ts (root: U32.t{0 < U32.v root}) = ts: tree_state_wf{
+  partial_wf ts root
+}
+
+/// Determine if the index is a non-leaf index in the heap.
+let is_internal_index (ts: tree_state_wf) (i: U32.t) =
+  0 < U32.v i /\ U32.v i <= ts.heap_len / 2
+
+/// The heap area is not empty.
+unfold let heap_not_empty (ts: tree_state_wf) = 0 < ts.heap_len
+
+/// The sorted area is empty.
+unfold let sorted_not_empty (ts: tree_state_wf) = ts.heap_max < U32.v heap_size
+
+/// Get the sorted area sequence.
+let sorted_seq (ts: tree_state_wf): Ghost (Seq.seq U32.t)
+  (requires ts.heap_max <= U32.v heap_size)
+  (ensures fun s -> Seq.length s == U32.v heap_size - ts.heap_max) =
+  Seq.slice ts.heap ts.heap_max (U32.v heap_size)
+
+/// Get the heap area sequence.
+let heap_seq (ts: tree_state_wf): Ghost (Seq.seq U32.t)
+  (requires heap_not_empty ts /\ heap_indexes_wf ts)
+  (ensures fun s -> Seq.length s == ts.heap_len) =
+  Seq.slice ts.heap 1 (ts.heap_len + 1)
+
+/// Get the concatenation of the heap area and sorted area.
+let element_seq (ts: tree_state_wf): Ghost (Seq.seq U32.t)
+  (requires heap_not_empty ts /\ heap_indexes_wf ts)
+  (ensures fun s ->
+    Seq.length s == ts.heap_len + U32.v heap_size - ts.heap_max) =
+  heap_seq ts @| sorted_seq ts
+
+/// Non-heap areas are not modified.
+let non_heap_unmodified (h1 h2: seq U32.t) (heap_len: nat) =
+  forall i. {:pattern (h1.[i]) \/ (h2.[i])} (i = 0 \/ i > heap_len) ==> h1.[i] == h2.[i]
+
+/// The elements in the sorted area are sorted.
+private let rec heap_sorted' (ts: heap_elems_wf_ts) (i: nat{
+  ts.heap_max <= i /\ i <= U32.v heap_size
+}): GTot bool
+  (decreases U32.v heap_size - i) =
+  let heap = ts.heap in
+  if U32.v heap_size - i <= 1 then
+    true
+  else if smaller ts heap.[i + 1] heap.[i] then
+    heap_sorted' ts (i + 1)
+  else
+    false
+
+unfold let heap_sorted (ts: heap_elems_wf_ts) = heap_sorted' ts ts.heap_max
+
+/// The first element in the sorted area is smaller than all elements in the heap.
+unfold let sorted_lt_heap (ts: heap_elems_wf_ts) =
+  sorted_not_empty ts ==> (forall i. 1 <= i /\ i <= ts.heap_len ==>
+    smaller ts ts.heap.[ts.heap_max] ts.heap.[i])
+
+/// Heap well-formed tree status. The heap is complete well-formed, which root
+/// element is the smallest element in the heap area. Elements in the sorted area
+/// are sorted as well, and the tree status should satisfy with sorted_lt_heap as
+/// well.
+unfold let heap_wf (ts: tree_state_wf) =
+  partial_wf ts 1ul /\ heap_sorted ts /\ heap_not_empty ts /\ sorted_lt_heap ts
+  
+type heap_wf_ts = ts: tree_state_wf{heap_wf ts}
+
+/// At the end of the do_pqdownheap call, the two heap areas of ts0 and ts1 should
+/// be a permutation after the assignment.
+private val lemma_heap_seq_upd_perm:
+    ts0: heap_elems_wf_ts{heap_not_empty ts0}
+  -> ts1: heap_elems_wf_ts{ts1 == {ts0 with heap = ts1.heap}}
+  -> Lemma
+  (requires
+    permutation U32.t ts0.heap ts1.heap /\
+    non_heap_unmodified ts0.heap ts1.heap ts0.heap_len)
+  (ensures permutation U32.t (heap_seq ts0) (heap_seq ts1))
+  [SMTPat (permutation U32.t (heap_seq ts0) (heap_seq ts1))]
+
+private val lemma_non_heap_unmodified:
+    ts0: heap_elems_wf_ts
+  -> ts1: heap_elems_wf_ts
+  -> Lemma
+  (requires
+    ts1 == {ts0 with heap = ts1.heap} /\
+    non_heap_unmodified ts0.heap ts1.heap ts0.heap_len /\
+    heap_sorted ts0)
+  (ensures heap_sorted ts1 /\ sorted_seq ts0 == sorted_seq ts1)
+  [SMTPatOr [
+    [SMTPat (heap_sorted ts0); SMTPat (heap_sorted ts1)];
+    [SMTPat (sorted_seq ts0); SMTPat (sorted_seq ts1)]
+  ]]
+
+type heap_area_wf_ts = partial_wf_ts 1ul
+
+/// If a heap is well-formed, its elements should not larger than the root.
+val lemma_heap_wf: ts: partial_wf_ts 1ul -> j: pos{j <= ts.heap_len} -> Lemma
+  (ensures smaller ts ts.heap.[1] ts.heap.[j])
+
+let lemma_heap_wf_forall (ts: partial_wf_ts 1ul): Lemma
+  (ensures forall j. 0 < j /\ j <= ts.heap_len ==>
+    smaller ts ts.heap.[1] ts.heap.[j]) =
+  let open FStar.Classical in
+  forall_intro (move_requires (lemma_heap_wf ts))
+
+/// Move the root element from the heap area to the top of sorted area will keep
+/// area sorted.
+val lemma_heap_wf_pqremove: ts: heap_wf_ts -> Lemma
+  (requires ts.heap_len > 1)
+  (ensures (
+    let ts' = {
+      ts with
+      heap = upd (upd ts.heap (ts.heap_max - 1) ts.heap.[1]) 1 ts.heap.[ts.heap_len];
+      heap_max = ts.heap_max - 1;
+      heap_len = ts.heap_len - 1;
+    } in
+    heap_sorted ts' /\
+    sorted_lt_heap ts' /\
+    permutation U32.t (element_seq ts) (element_seq ts')))
