specs/Spec.Tree.Heap.fst
@@ -1,0 +1,250 @@
+module Spec.Tree.Heap
+
+module B = LowStar.Buffer
+module CB = LowStar.ConstBuffer
+module HS = FStar.HyperStack
+module U16 = FStar.UInt16
+module U32 = FStar.UInt32
+module U8 = FStar.UInt8
+
+open FStar.Mul
+open FStar.Seq
+open Lib.Seq
+open Yazi.Tree.Types
+open Yazi.Deflate.Constants
+include Spec.Heap.Lemmas
+
+/// Live tree states definition.
+let tree_state_live (h: HS.mem) (ts: tree_state_t) =
+  (* The sorting context pointer should be live and its length should be one. *)
+  CB.live h ts.ctx /\ B.g_is_null (CB.as_mbuf ts.ctx) == false /\ CB.length ts.ctx == 1 /\
+  (let ctx' = (CB.as_seq h ts.ctx).[0] in
+  B.live h ctx'.state /\
+  (let heap_len = U32.v (B.as_seq h ctx'.state).[0] in
+  let heap_max = U32.v (B.as_seq h ctx'.state).[1] in
+  let heap = B.as_seq h ctx'.heap in
+  let tree = B.as_seq h ctx'.tree in
+  let depth = B.as_seq h ctx'.depth in
+  (* All three buffers should be live and disjoint with each other. *)
+  B.live h ctx'.heap /\ B.live h ctx'.tree /\ B.live h ctx'.depth /\
+  ~ (B.g_is_null ctx'.heap) /\ ~ (B.g_is_null ctx'.tree) /\ ~ (B.g_is_null ctx'.depth) /\
+
+  (let ctx = CB.as_mbuf ts.ctx in
+  B.disjoint ctx ctx'.state /\ B.disjoint ctx ctx'.tree /\ B.disjoint ctx ctx'.heap /\
+  B.disjoint ctx ctx'.depth /\ B.disjoint ctx'.state ctx'.tree /\
+  B.disjoint ctx'.state ctx'.heap /\ B.disjoint ctx'.state ctx'.depth /\
+  B.disjoint ctx'.tree ctx'.heap /\ B.disjoint ctx'.tree ctx'.depth /\
+  B.disjoint ctx'.heap ctx'.depth) /\
+
+  (* The length of the tree buffer should equal to the tree_len. *)
+  B.length ctx'.tree == Ghost.reveal ts.tree_len))
+
+type live_tree_state (h: HS.mem) = s: tree_state_t{
+  tree_state_live h s
+}
+
+/// Convert the C struct to specification record type.
+let g_tree_state (h: HS.mem) (ts: live_tree_state h): GTot (res: tree_state_wf{
+  let ctx = (CB.as_seq h ts.ctx).[0] in
+  res.heap_len == U32.v (B.as_seq h ctx.state).[0] /\
+  res.heap_max == U32.v (B.as_seq h ctx.state).[1] /\
+  res.tree_len == Ghost.reveal ((ts <: tree_state_t).tree_len)
+}) =
+  let ctx = (CB.as_seq h ts.ctx).[0] in {
+    heap = B.as_seq h ctx.heap;
+    tree = B.as_seq h ctx.tree;
+    depth = B.as_seq h ctx.depth;
+    heap_len = U32.v (B.as_seq h ctx.state).[0];
+    heap_max = U32.v (B.as_seq h ctx.state).[1];
+    tree_len = Ghost.reveal (ts <: tree_state_t).tree_len;
+    forest = Ghost.reveal (ts <: tree_state_t).forest;
+  }
+  
+/// Getter for heap_len and heap_max.
+unfold let get_heap_len (h: HS.mem) (ts: live_tree_state h) =
+  (g_tree_state h ts).heap_len
+
+unfold let get_heap_max (h: HS.mem) (ts: live_tree_state h) =
+  (g_tree_state h ts).heap_max
+  
+/// Pre-condition before i is inserted to the heap.
+let insertion_pre_cond (ts: heap_elems_wf_ts) (root i hole: U32.t) =
+  let open U32 in
+  let heap = ts.heap in
+  is_tree_index ts i /\
+  is_internal_index ts root /\
+  U32.v root <= U32.v hole /\ U32.v hole <= ts.heap_len /\
+  heap_not_empty ts /\
+    
+  (* heap.[v hole] `smaller` i *)
+  smaller ts heap.[U32.v hole] i /\
+
+  (* Initial state, elements after root form a partial heap and i is in the root. *)
+  (root == hole ==> partial_wf ts (root +^ 1ul) /\ heap.[v root] == i) /\
+
+  (* Intermediate state, elements start from root form a partial heap.
+     The element i has not been inserted to the partial heap. *)
+  (v root < v hole ==> partial_wf ts root)
+
+/// Determine the smallest element among i, heap[hole * 2], and heap[hole * 2 + 1]
+/// (if the right child of hole exists). If i is the smallest element, then we can
+/// insert i into heap[hole] because heap[hole / 2] == heap[hole] or hole == root.
+let smallest (ts: heap_elems_wf_ts) (root i hole: U32.t): Ghost U32.t 
+  (requires
+    insertion_pre_cond ts root i hole /\
+    U32.v hole <= ts.heap_len / 2)
+  (ensures fun res ->
+    let res = U32.v res in
+    let root = U32.v root in
+    let hole = U32.v hole in
+    let heap = ts.heap in
+    let smaller = smaller ts in
+
+    (* The returned result should be zero or hole's child.*)
+    res <= ts.heap_len /\
+    (res == 0 \/ res == hole * 2 \/ res == hole * 2 + 1) /\
+
+    (* If the result is zero then i is the smallest element among i, the left
+       child of hole, and the right child of hole (if it exists). *)
+    (let k = if res = 0 then i else heap.[res] in
+    (* The index should be the smallest one among the three indexes. *)
+    k `smaller` i /\
+    k `smaller` heap.[hole * 2] /\
+    (hole * 2 + 1 <= ts.heap_len ==> k `smaller` heap.[hole * 2 + 1]) /\
+    
+    (root == hole ==> k `smaller` heap.[hole]) /\
+    (root < hole ==> heap.[hole] `smaller` k) /\
+    res > 0 ==> res > hole)) =
+  let open U32 in
+  let smaller = smaller ts in
+  let heap = ts.heap in
+  let l = hole *^ 2ul in let r = l +^ 1ul in
+  let le = heap.[v l] in
+  
+  if v r > ts.heap_len then
+    if i `smaller` le then 0ul else l
+  else
+    let re = heap.[v r] in
+    if i `smaller` le then
+      if i `smaller` re then 0ul else r
+    else
+      if le `smaller` re then l else r
+
+/// Count invariant during the do_pqdownheap iteration. After the iteration,
+/// this invariant will not hold and partial_wf will hold after the end of the
+/// iteration.
+let count_inv (h1 h2: seq U32.t) (root i hole: U32.t) =
+  let root = U32.v root in let hole = U32.v hole in
+  (* h1 is the initial heap and the root of h1 is the element to be inserted to
+     the heap.*)
+  length h1 == length h2 /\
+  root <= hole /\ hole < length h1 /\
+
+  (* At the beginning, the new element is in the root. *)
+  h1.[root] == i /\
+
+  (* If we haven't done anything on h2, they should be the same.*)
+  (hole == root ==> h1 == h2) /\
+  
+  (hole <> root ==> 
+    (* Intermediate state. *)
+    (h2.[hole] <> h1.[root] ==>
+      (* The count of the root element in h2 is one less than h1 because h2.[root]
+         is replaced with a smaller child. *)
+      count h1.[root] h2 + 1 == count h1.[root] h1 /\
+      (* Conversely, since h2.[hole / 2] == h2.[hole], so we have one more h2.[hole]
+         in h2. *)
+      count h2.[hole] h2 == count h2.[hole] h1 + 1) /\
+
+    (* If they are equal, then there the previous do_pqdownheap iteration did not
+       change the count of the root element. *)
+    (h2.[hole] == h1.[root] ==> count h1.[root] h2 == count h1.[root] h1) /\
+    
+    (* For other elements, thier counts are unchanged. *)
+    (forall (x: U32.t). {:pattern (count x h1) \/ (count x h2)}
+      x <> h1.[root] /\ x <> h2.[hole] ==> count x h1 == count x h2))
+
+let do_pqdownheap_pre (ts0 ts1: tree_state_wf) (root i hole: U32.t) =
+  let heap0 = ts0.heap in
+  let heap1 = ts1.heap in
+  let heap_len = ts1.heap_len in
+  heap_elems_wf ts0 /\ heap_elems_wf ts1 /\
+  ts1 == {ts0 with heap = ts1.heap} /\
+  insertion_pre_cond ts1 root i hole /\
+  count_inv heap0 heap1 root i hole /\
+  non_heap_unmodified heap0 heap1 heap_len /\
+  (U32.v root == 1 ==> heap_sorted ts1 /\ sorted_lt_heap ts1)
+
+#push-options "--z3refresh --z3rlimit 256 --fuel 0 --ifuel 0 --z3seed 111"
+let rec do_pqdownheap
+  (ts0 ts1: heap_elems_wf_ts)
+  (root: U32.t{0 < U32.v root}) (i hole: U32.t):
+  Ghost (partial_wf_ts root)
+  (requires do_pqdownheap_pre ts0 ts1 root i hole)
+  (ensures fun ts2 ->
+     ts2 == {ts1 with heap = ts2.heap} /\
+     non_heap_unmodified ts1.heap ts2.heap ts2.heap_len /\
+     permutation U32.t ts0.heap ts2.heap /\
+     permutation U32.t (heap_seq ts0) (heap_seq ts2) /\
+     sorted_seq ts1 == sorted_seq ts2 /\
+     (U32.v root == 1 ==> heap_wf ts2))
+  (decreases ts1.heap_len - U32.v hole) =
+  let open U32 in
+  if v hole > ts1.heap_len / 2 then
+    {ts1 with heap = upd ts1.heap (v hole) i}
+  else
+    let s = smallest ts1 root i hole in
+    if s = 0ul then
+      {ts1 with heap = upd ts1.heap (v hole) i}
+    else
+      let ts1' = {ts1 with heap = upd ts1.heap (v hole) ts1.heap.[v s]} in
+      do_pqdownheap ts0 ts1' root i s
+#pop-options
+
+unfold let pqdownheap_pre (ts: tree_state_wf) (i: U32.t{is_internal_index ts i}) =
+  heap_elems_wf ts /\
+  partial_wf ts (i `U32.add` 1ul) /\
+  (U32.v i == 1 ==> heap_sorted ts /\ sorted_lt_heap ts)
+
+/// Move the root element to keep heap's invariant.
+let pqdownheap (ts: tree_state_wf) (i: U32.t{is_internal_index ts i}):
+  Ghost (partial_wf_ts i)
+  (requires pqdownheap_pre ts i)
+  (ensures fun ts' ->
+    ts' = {ts with heap = ts'.heap} /\
+    non_heap_unmodified ts.heap ts'.heap ts.heap_len /\
+    permutation U32.t ts.heap ts'.heap /\
+    permutation U32.t (heap_seq ts) (heap_seq ts') /\
+    sorted_seq ts == sorted_seq ts' /\
+    permutation U32.t (element_seq ts) (element_seq ts') /\
+    (U32.v i == 1 ==> heap_wf ts')) =
+  let ts' = do_pqdownheap ts ts i ts.heap.[U32.v i] i in
+  lemma_append_count (heap_seq ts) (sorted_seq ts);
+  lemma_append_count (heap_seq ts') (sorted_seq ts');
+  ts'
+
+#push-options "--z3refresh --z3rlimit 256 --fuel 1 --ifuel 1"
+/// Move the root of the heap to the sorted area.
+let pqremove (ts: heap_wf_ts):
+  Ghost heap_wf_ts
+  (requires ts.heap_len > 1)
+  (ensures fun ts' ->
+    ts' == {
+      ts with
+      heap = ts'.heap;
+      heap_len = ts.heap_len - 1;
+      heap_max = ts.heap_max - 1;
+    } /\
+    permutation U32.t (element_seq ts) (element_seq ts')) =
+  lemma_heap_wf_pqremove ts;
+  let ts1 = {
+    ts with
+    heap = upd (upd ts.heap (ts.heap_max - 1) ts.heap.[1]) 1 ts.heap.[ts.heap_len];
+    heap_len = ts.heap_len - 1;
+    heap_max = ts.heap_max - 1;
+  } in
+  if ts1.heap_len >= 2 then
+    pqdownheap ts1 1ul
+  else
+    ts1
+#pop-options
